Beginning of splitting into appropriate modules

common/theories/LoopChecking/PartialLoopChecking.v
@@ -6,93 +6,16 @@ From MetaRocq.Utils Require Import utils.
 
 From MetaRocq.Common Require Universes.
 From Equations Require Import Equations.
+
+From MetaRocq.Common.LoopChecking Require Import Common Interfaces.
+
 Set Equations Transparent.
 
-Ltac rw l := rewrite_strat (topdown l).
-Ltac rw_in l H := rewrite_strat (topdown l) in H.
-
-
-(* TODO move *)
-Arguments exist {A P}.
-Definition inspect {A} (x : A) : { y : A | x = y } := exist x eq_refl.
-
-Module FMapOrderedType_from_UsualOrderedType (O : UsualOrderedType).
-  Import O.
-  Definition t := O.t.
-  Definition eq : O.t -> O.t -> Prop := O.eq.
-  Definition lt : O.t -> O.t -> Prop := O.lt.
-  Definition eq_refl : forall x : O.t, eq x x := reflexivity.
-  Definition eq_sym : forall x y : O.t, eq x y -> eq y x := fun x y H => symmetry H.
-
-  Lemma eq_trans : forall x y z, O.eq x y -> O.eq y z -> O.eq x z.
-  Proof. intros x y z. unfold O.eq. apply transitivity. Qed.
-  Lemma lt_trans : forall x y z, O.lt x y -> O.lt y z -> O.lt x z.
-  Proof. intros. eapply O.lt_strorder; tea. Qed.
-
-  Lemma lt_not_eq : forall x y : O.t, lt x y -> ~ eq x y.
-  Proof.
-    intros x y H eq. do 2 red in eq. subst x. now eapply lt_strorder in H.
-  Qed.
-
-  Definition compare : forall x y : O.t, Compare lt eq x y.
-  Proof.
-    intros.
-    case_eq (compare x y); intros.
-    apply EQ. abstract (destruct (compare_spec x y) => //).
-    apply LT. abstract (destruct (compare_spec x y) => //).
-    apply GT. abstract (destruct (compare_spec x y) => //).
-  Defined.
-
-  Definition eq_dec : forall x y : O.t, {eq x y} + {~ eq x y} := eq_dec.
-End FMapOrderedType_from_UsualOrderedType.
-
-Module Type LevelOrderedType.
-  Include UsualOrderedType.
-
-  Parameter reflect_eq : ReflectEq t.
-  #[local] Existing Instance reflect_eq.
-  Parameter eq_leibniz : forall (x y : t), eq x y -> x = y.
-
-  Parameter to_string : t -> string.
-
-End LevelOrderedType.
-
-Module Type FMapOTInterface (E : UsualOrderedType).
-  Module OT := FMapOrderedType_from_UsualOrderedType E.
-  Include FMapInterface.Sfun OT.
-End FMapOTInterface.
-
-Module Type LevelSet_fun (Level : LevelOrderedType).
-  Include SWithLeibniz with Module E := Level.
-End LevelSet_fun.
-
-Module Type LevelExprItf (Level : LevelOrderedType).
-  Include UsualOrderedType with Definition t := (Level.t * Z)%type.
-  Parameter eq_leibniz : forall (x y : t), eq x y -> x = y.
-End LevelExprItf.
-
-Module Type LevelExprSet_fun (Level : LevelOrderedType) (LevelExpr : LevelExprItf Level).
-  Include SWithLeibniz with Module E := LevelExpr.
-
-  Record nonEmptyLevelExprSet
-    := { t_set :> t ;
-          t_ne  : is_empty t_set = false }.
-
-  (* Parameter map : (LevelExpr.t -> LevelExpr.t) -> nonEmptyLevelExprSet -> nonEmptyLevelExprSet. *)
-
-  (* Parameter map_spec : forall e f u, In e (map f u) <-> exists e0, In e0 u /\ e = (f e0). *)
-
-End LevelExprSet_fun.
-
-Module Type LoopCheckingItf (Level : LevelOrderedType)
-  (LevelSet : LevelSet_fun Level)
-  (LevelExpr : LevelExprItf Level)
-  (LevelExprSet : LevelExprSet_fun Level LevelExpr)
-  (LevelMap : FMapOTInterface Level).
+Module Type LoopCheckingItf (LS : LevelSets).
 
   (* Type of consistent models of a set of universe constraints *)
   Parameter model : Type.
-  Notation univ := LevelExprSet.nonEmptyLevelExprSet.
+  Notation univ := LS.LevelExprSet.nonEmptyLevelExprSet.
 
   Inductive constraint_type := UnivEq | UnivLe.
   Notation constraint := (univ * constraint_type * univ).
@@ -100,7 +23,7 @@ Module Type LoopCheckingItf (Level : LevelOrderedType)
   Parameter init_model : model.
 
   (* Returns None if already declared *)
-  Parameter declare_level : Level.t -> model -> option model.
+  Parameter declare_level : LS.Level.t -> model -> option model.
 
   (* If the constraints mention undeclared universes, returns None,
      otherwise, returns either a model or a looping universe, i.e. such that u >= u + 1 is implied
@@ -114,356 +37,11 @@ Module Type LoopCheckingItf (Level : LevelOrderedType)
 
   (* Returns the valuation of the model: a minimal assignement from levels to constraints
     that make the enforced clauses valid. *)
-  Parameter valuation : model -> LevelMap.t nat.
-
+  Parameter valuation : model -> LS.LevelMap.t nat.
 End LoopCheckingItf.
 
-Module LoopCheckingImpl
-  (* Signature of levels: decidable, ordered type *)
-  (Level : LevelOrderedType)
-  (LevelSet : LevelSet_fun Level)
-  (LevelExpr : LevelExprItf Level)
-  (LevelExprSet : LevelExprSet_fun Level LevelExpr)
-  (LevelMap : FMapOTInterface Level).
-
-Definition level (e : LevelExpr.t) : Level.t := fst e.
-Definition levels (e : LevelExprSet.t) :=
-  LevelExprSet.fold (fun le => LevelSet.add (level le)) e LevelSet.empty.
-  Import LevelExprSet (nonEmptyLevelExprSet, t_set, t_ne).
-
-
-Local Existing Instance Level.reflect_eq.
-
-Module LevelSetFact := WFactsOn Level LevelSet.
-Module LevelSetProp := WPropertiesOn Level LevelSet.
-Module LevelSetDecide := LevelSetProp.Dec.
-Module LevelMapFact := FMapFacts.WProperties_fun LevelMap.OT LevelMap.
-
-Ltac lsets := LevelSetDecide.fsetdec.
-Notation "(=_lset)" := LevelSet.Equal (at level 0).
-Infix "=_lset" := LevelSet.Equal (at level 30).
-Infix "⊂_lset" := LevelSet.Subset (at level 70).
-Infix "∪" := LevelSet.union (at level 70).
-
-Definition print_level_nat_map (m : LevelMap.t nat) :=
-  let list := LevelMap.elements m in
-  print_list (fun '(l, w) => Level.to_string l ^ " -> " ^ string_of_nat w) nl list.
-
-Definition print_lset (l : LevelSet.t) :=
-  let list := LevelSet.elements l in
-  print_list Level.to_string " " list.
-
-Module LevelExprSetFact := WFactsOn LevelExpr LevelExprSet.
-Module LevelExprSetProp := WPropertiesOn LevelExpr LevelExprSet.
-
-(* We have decidable equality w.r.t leibniz equality for sets of levels. *)
-#[global, program] Instance levelexprset_reflect : ReflectEq LevelExprSet.t :=
-  { eqb := LevelExprSet.equal }.
-Next Obligation.
-  destruct (LevelExprSet.equal x y) eqn:e; constructor.
-  eapply LevelExprSet.equal_spec in e.
-  now eapply LevelExprSet.eq_leibniz.
-  intros e'.
-  subst y.
-  pose proof (@LevelExprSetFact.equal_1 x x).
-  forward H. reflexivity. congruence.
-Qed.
-
-#[global] Instance levelexprset_eq_dec : Classes.EqDec LevelExprSet.t := Classes.eq_dec.
-
-Derive NoConfusion for LevelExprSet.nonEmptyLevelExprSet.
-
-(* We use uip on the is_empty condition *)
-#[global, program] Instance nonEmptyLevelExprSet_reflect : ReflectEq nonEmptyLevelExprSet :=
-  { eqb x y := eqb x.(t_set) y.(t_set) }.
-Next Obligation.
-  destruct (eqb_spec (t_set x) (t_set y)); constructor.
-  destruct x, y; cbn in *. subst.
-  now rewrite (uip t_ne0 t_ne1).
-  intros e; subst x; apply H.
-  reflexivity.
-Qed.
-
-(** This coercion allows to see the non-empty set as a regular [LevelExprSet.t] *)
-Coercion t_set : nonEmptyLevelExprSet >-> LevelExprSet.t.
-Module LevelExprSetDecide := WDecide (LevelExprSet).
-Ltac lesets := LevelExprSetDecide.fsetdec.
-Infix "⊂_leset" := LevelExprSet.Subset (at level 70).
-
-Lemma levelset_not_Empty_is_empty s :
-  LevelSet.is_empty s = false <-> ~ LevelSet.Empty s.
-Proof.
-  split.
-  - intros H he. red in he. apply negbT in H. unshelve eapply (contraNnot _ H).
-    3:exact he. intros ha. now apply LevelSetFact.is_empty_1.
-  - intros ne. destruct LevelSet.is_empty eqn:he => //.
-    eapply LevelSetFact.is_empty_2 in he. contradiction.
-Qed.
-
-Module NonEmptySetFacts.
-  #[program] Definition singleton (e : LevelExpr.t) : nonEmptyLevelExprSet
-    := {| t_set := LevelExprSet.singleton e |}.
-  Next Obligation.
-    apply negbTE.
-    eapply (contra_notN (P := LevelExprSet.Empty (LevelExprSet.singleton e))).
-    apply LevelExprSetFact.is_empty_2. intros ne. red in ne. specialize (ne e). lesets.
-  Qed.
-
-  Lemma not_Empty_is_empty s :
-    ~ LevelExprSet.Empty s <-> LevelExprSet.is_empty s = false.
-  Proof.
-    split.
-    - intro H. apply not_true_is_false. intro H'.
-      apply H. now apply LevelExprSetFact.is_empty_2 in H'.
-    - intros H he. red in he. apply negbT in H. unshelve eapply (contraNnot _ H).
-      3:exact he. intros ha. now apply LevelExprSetFact.is_empty_1.
-  Qed.
-
-  Program Definition add (e : LevelExpr.t) (u : nonEmptyLevelExprSet) : nonEmptyLevelExprSet
-    := {| t_set := LevelExprSet.add e u |}.
-  Next Obligation.
-    apply not_Empty_is_empty; intro H.
-    eapply H. eapply LevelExprSet.add_spec.
-    left; reflexivity.
-  Qed.
-
-  Lemma add_spec e u e' :
-    LevelExprSet.In e' (add e u) <-> e' = e \/ LevelExprSet.In e' u.
-  Proof.
-    apply LevelExprSet.add_spec.
-  Qed.
-
-  Definition add_list : list LevelExpr.t -> nonEmptyLevelExprSet -> nonEmptyLevelExprSet
-    := List.fold_left (fun u e => add e u).
-
-  Lemma add_list_spec l u e :
-    LevelExprSet.In e (add_list l u) <-> In e l \/ LevelExprSet.In e u.
-  Proof.
-    unfold add_list. rewrite <- fold_left_rev_right.
-    etransitivity. 2:{ eapply or_iff_compat_r. etransitivity.
-                        2: apply @InA_In_eq with (A:=LevelExpr.t).
-                        eapply InA_rev. }
-    induction (List.rev l); cbn.
-    - split. intuition. intros [H|H]; tas. invs H.
-    - split.
-      + intro H. apply add_spec in H. destruct H as [H|H].
-        * left. now constructor.
-        * apply IHl0 in H. destruct H as [H|H]; [left|now right].
-          now constructor 2.
-      + intros [H|H]. inv H.
-        * apply add_spec; now left.
-        * apply add_spec; right. apply IHl0. now left.
-        * apply add_spec; right. apply IHl0. now right.
-  Qed.
-
-  Lemma elements_not_empty {u : nonEmptyLevelExprSet} : LevelExprSet.elements u <> [].
-  Proof.
-    rewrite -LevelExprSetProp.elements_Empty.
-    move/LevelExprSetFact.is_empty_1.
-    destruct u as [u1 u2]; cbn in *. congruence.
-  Qed.
-
-  Equations to_nonempty_list (u : nonEmptyLevelExprSet) : LevelExpr.t * list LevelExpr.t :=
-  | u with inspect (LevelExprSet.elements u) := {
-    | exist [] eqel => False_rect _ (elements_not_empty eqel)
-    | exist (e :: l) _ => (e, l) }.
-
-  Lemma singleton_to_nonempty_list e : to_nonempty_list (singleton e) = (e, []).
-  Proof.
-    funelim (to_nonempty_list (singleton e)). bang.
-    clear H.
-    pose proof (LevelExprSet.singleton_spec e1 e).
-    rewrite LevelExprSetFact.elements_iff in H.
-    rewrite InA_In_eq in H. rewrite e0 in H.
-    destruct H. forward H. now left. noconf H. f_equal.
-    pose proof (LevelExprSet.cardinal_spec (LevelExprSet.singleton e1)). rewrite e0 in H. cbn in H.
-    rewrite LevelExprSetProp.singleton_cardinal in H.
-    destruct l => //.
-  Qed.
-
-  Lemma to_nonempty_list_spec u :
-    let '(e, u') := to_nonempty_list u in
-    e :: u' = LevelExprSet.elements u.
-  Proof.
-    funelim (to_nonempty_list u). bang. now rewrite e0.
-  Qed.
-
-  Lemma to_nonempty_list_spec' u :
-    (to_nonempty_list u).1 :: (to_nonempty_list u).2 = LevelExprSet.elements u.
-  Proof.
-    pose proof (to_nonempty_list_spec u).
-    now destruct (to_nonempty_list u).
-  Qed.
-
-  Lemma In_to_nonempty_list (u : nonEmptyLevelExprSet) (e : LevelExpr.t) :
-    LevelExprSet.In e u
-    <-> e = (to_nonempty_list u).1 \/ In e (to_nonempty_list u).2.
-  Proof.
-    etransitivity. symmetry. apply LevelExprSet.elements_spec1.
-    pose proof (to_nonempty_list_spec' u) as H.
-    destruct (to_nonempty_list u) as [e' l]; cbn in *.
-    rewrite <- H; clear. etransitivity. apply InA_cons.
-    eapply or_iff_compat_l. apply InA_In_eq.
-  Qed.
-
-  Lemma In_to_nonempty_list_rev (u : nonEmptyLevelExprSet) (e : LevelExpr.t) :
-    LevelExprSet.In e u
-    <-> e = (to_nonempty_list u).1 \/ In e (List.rev (to_nonempty_list u).2).
-  Proof.
-    etransitivity. eapply In_to_nonempty_list.
-    apply or_iff_compat_l. apply in_rev.
-  Qed.
-
-  Program Definition map (f : LevelExpr.t -> LevelExpr.t) (u : nonEmptyLevelExprSet) : nonEmptyLevelExprSet :=
-    {| t_set := LevelExprSetProp.of_list (List.map f (LevelExprSet.elements u)) |}.
-  Next Obligation.
-    have hs := to_nonempty_list_spec u.
-    destruct (to_nonempty_list u). rewrite -hs. cbn.
-    apply not_Empty_is_empty => he. apply (he (f t)).
-    lesets.
-  Qed.
-
-  Lemma map_spec f u e :
-    LevelExprSet.In e (map f u) <-> exists e0, LevelExprSet.In e0 u /\ e = (f e0).
-  Proof.
-    unfold map; cbn.
-    rewrite LevelExprSetProp.of_list_1 InA_In_eq in_map_iff.
-    split.
-    - intros [x [<- hin]]. exists x. split => //.
-      rewrite -InA_In_eq in hin. now apply LevelExprSet.elements_spec1 in hin.
-    - intros [x [hin ->]]. exists x. split => //.
-      rewrite -InA_In_eq. now apply LevelExprSet.elements_spec1.
-  Qed.
-
-  Program Definition non_empty_union (u v : nonEmptyLevelExprSet) : nonEmptyLevelExprSet :=
-    {| t_set := LevelExprSet.union u v |}.
-  Next Obligation.
-    apply not_Empty_is_empty; intro H.
-    assert (HH: LevelExprSet.Empty u). {
-      intros x Hx. apply (H x).
-      eapply LevelExprSet.union_spec. now left. }
-    apply LevelExprSetFact.is_empty_1 in HH.
-    rewrite t_ne in HH; discriminate.
-  Qed.
-
-
-  Lemma eq_univ (u v : nonEmptyLevelExprSet) :
-    u = v :> LevelExprSet.t -> u = v.
-  Proof.
-    destruct u as [u1 u2], v as [v1 v2]; cbn. intros X; destruct X.
-    now rewrite (uip_bool _ _ u2 v2).
-  Qed.
-
-  Lemma eq_univ_equal (u v : nonEmptyLevelExprSet) :
-    LevelExprSet.Equal u v <-> u = v.
-  Proof.
-    split.
-    - intro H. now apply eq_univ, LevelExprSet.eq_leibniz.
-    - intros ->; reflexivity.
-  Qed.
-
-  Lemma eq_univ_elements (u v : nonEmptyLevelExprSet) :
-    LevelExprSet.elements u = LevelExprSet.elements v -> u = v.
-  Proof.
-    intro H. apply eq_univ.
-    destruct u as [u1 u2], v as [v1 v2]; cbn in *; clear u2 v2.
-    eapply LevelExprSet.eq_leibniz. red.
-    intros x. rewrite -!LevelExprSet.elements_spec1 H //.
-  Qed.
-
-  Lemma univ_expr_eqb_true_iff (u v : nonEmptyLevelExprSet) :
-    LevelExprSet.equal u v <-> u = v.
-  Proof.
-    split.
-    - intros.
-      apply eq_univ_equal. now apply LevelExprSet.equal_spec.
-    - intros ->. now apply LevelExprSet.equal_spec.
-  Qed.
-
-  Lemma univ_expr_eqb_comm (u v : nonEmptyLevelExprSet) :
-    LevelExprSet.equal u v <-> LevelExprSet.equal v u.
-  Proof.
-    transitivity (u = v). 2: transitivity (v = u).
-    - apply univ_expr_eqb_true_iff.
-    - split; apply eq_sym.
-    - split; apply univ_expr_eqb_true_iff.
-  Qed.
-
-
-  Lemma LevelExprSet_for_all_false f u :
-    LevelExprSet.for_all f u = false -> LevelExprSet.exists_ (negb ∘ f) u.
-  Proof.
-    intro H. rewrite LevelExprSetFact.exists_b.
-    rewrite LevelExprSetFact.for_all_b in H.
-    all: try now intros x y [].
-    induction (LevelExprSet.elements u); cbn in *; [discriminate|].
-    apply andb_false_iff in H; apply orb_true_iff; destruct H as [H|H].
-    left; now rewrite H.
-    right; now rewrite IHl.
-  Qed.
-
-  Lemma LevelExprSet_For_all_exprs (P : LevelExpr.t -> Prop) (u : nonEmptyLevelExprSet)
-    : LevelExprSet.For_all P u
-      <-> P (to_nonempty_list u).1 /\ Forall P (to_nonempty_list u).2.
-  Proof.
-    etransitivity.
-    - eapply iff_forall; intro e. eapply imp_iff_compat_r.
-      apply In_to_nonempty_list.
-    - cbn; split.
-      + intro H. split. apply H. now left.
-        apply Forall_forall. intros x H0.  apply H; now right.
-      + intros [H1 H2] e [He|He]. subst e; tas.
-        eapply Forall_forall in H2; tea.
-  Qed.
-
-  Lemma add_comm {le le' e} : add le (add le' e) = add le' (add le e).
-  Proof.
-    apply eq_univ_equal. intros x.
-    rewrite !LevelExprSet.add_spec. firstorder.
-  Qed.
-
-  #[program]
-  Definition univ_union (prems prems' : nonEmptyLevelExprSet) : nonEmptyLevelExprSet :=
-    {| t_set := LevelExprSet.union prems prems' |}.
-  Next Obligation.
-    destruct prems, prems'; cbn.
-    destruct (LevelExprSet.is_empty (LevelExprSet.union _ _)) eqn:ise => //.
-    eapply LevelExprSetFact.is_empty_2 in ise.
-    eapply not_Empty_is_empty in t_ne0, t_ne1.
-    destruct t_ne0. lesets.
-  Qed.
-
-  Lemma univ_union_spec u u' l :
-    LevelExprSet.In l (univ_union u u') <->
-    LevelExprSet.In l u \/ LevelExprSet.In l u'.
-  Proof.
-    destruct u, u'; unfold univ_union; cbn.
-    apply LevelExprSet.union_spec.
-  Qed.
-
-  Lemma univ_union_add_singleton u le : univ_union u (singleton le) = add le u.
-  Proof.
-    apply eq_univ_equal.
-    intros x. rewrite univ_union_spec LevelExprSet.singleton_spec add_spec.
-    intuition auto.
-  Qed.
-
-  Lemma univ_union_comm {u u'} : univ_union u u' = univ_union u' u.
-  Proof.
-    apply eq_univ_equal.
-    intros x. rewrite !univ_union_spec.
-    intuition auto.
-  Qed.
-
-  Lemma univ_union_add_distr {le u u'} : univ_union (add le u) u' = add le (univ_union u u').
-  Proof.
-    apply eq_univ_equal.
-    intros x. rewrite !univ_union_spec !add_spec !univ_union_spec.
-    intuition auto.
-  Qed.
-
-End NonEmptySetFacts.
-Import NonEmptySetFacts.
+Module LoopCheckingImpl (LS : LevelSets).
+  Module Import FLS := FromLevelSets(LS).
 
 Notation univ := nonEmptyLevelExprSet.
 Definition clause : Type := univ × LevelExpr.t.
@@ -574,10 +152,6 @@ Proof.
     rewrite Clauses.filter_spec. intuition auto.
 Qed.
 
-Definition levelexpr_level : LevelExpr.t -> Level.t := fst.
-Coercion levelexpr_level : LevelExpr.t >-> Level.t.
-Extraction Inline levelexpr_level.
-
 Definition strict_subset (s s' : LevelSet.t) :=
   LevelSet.Subset s s' /\ ~ LevelSet.Equal s s'.
 
@@ -608,7 +182,7 @@ Definition concl (cl : clause) := snd cl.
 Extraction Inline premise concl.
 
 Definition clause_levels cl :=
-  LevelSet.union (levels (premise cl)) (LevelSet.singleton (levelexpr_level (concl cl))).
+  LevelSet.union (levels (premise cl)) (LevelSet.singleton (level (concl cl))).
 
 Definition clauses_levels (cls : clauses) : LevelSet.t :=
   Clauses.fold (fun cl acc => LevelSet.union (clause_levels cl) acc) cls LevelSet.empty.
@@ -661,13 +235,13 @@ Qed.
 
 Lemma clause_levels_spec l cl :
   LevelSet.In l (clause_levels cl) <->
-  LevelSet.In l (levels (premise cl)) \/ l = levelexpr_level (concl cl).
+  LevelSet.In l (levels (premise cl)) \/ l = level (concl cl).
 Proof.
   unfold clause_levels.
   now rewrite LevelSet.union_spec LevelSet.singleton_spec.
 Qed.
 
-Definition clause_conclusion cl := levelexpr_level (concl cl).
+Definition clause_conclusion cl := level (concl cl).
 
 Local Open Scope Z_scope.
 
@@ -680,7 +254,7 @@ Definition level_value (m : model) (level : Level.t) : option Z :=
   end.
 
 Definition levelexpr_value (m : model) (atom : LevelExpr.t) :=
-  level_value m (levelexpr_level atom).
+  level_value m (level atom).
 
 Extraction Inline levelexpr_value.
 
@@ -1229,22 +803,16 @@ Definition v_minus_w_bound (W : LevelSet.t) (m : model) :=
   LevelMap.fold (fun w v acc => Z.max (option_get 0 v) acc)
     (LevelMapFact.filter (fun l _ => ~~ LevelSet.mem l W) m) 0%Z.
 
-Definition levelexpr_k : LevelExpr.t -> Z := snd.
-Coercion levelexpr_k : LevelExpr.t >-> Z.
-
-Definition level_expr_elt : LevelExprSet.elt -> LevelExpr.t := fun x => x.
-Coercion level_expr_elt : LevelExprSet.elt >-> LevelExpr.t.
-
 Definition premise_min (l : nonEmptyLevelExprSet) : Z :=
   let (hd, tl) := NonEmptySetFacts.to_nonempty_list l in
-  fold_left (B:=LevelExpr.t) (fun min atom => Z.min atom min) tl hd.
+  fold_left (B:=LevelExpr.t) (fun min atom => Z.min atom.2 min) tl (hd.2).
 
 Definition premise_max (l : nonEmptyLevelExprSet) : Z :=
   let (hd, tl) := NonEmptySetFacts.to_nonempty_list l in
-  fold_left (B:=LevelExpr.t) (fun min atom => Z.max atom min) tl hd.
+  fold_left (B:=LevelExpr.t) (fun min atom => Z.max atom.2 min) tl (hd.2).
 
 Definition gain (cl : clause) : Z :=
-  (levelexpr_k (concl cl)) - (premise_min (premise cl)).
+  (concl cl).2 - (premise_min (premise cl)).
 
 Definition max_gain (cls : clauses) :=
   Clauses.fold (fun cl acc => Nat.max (Z.to_nat (gain cl)) acc) cls 0%nat.
@@ -1719,7 +1287,7 @@ Proof.
     rewrite LevelSet.add_spec.
     split.
     * intros [->|].
-      left. exists (levelexpr_k x). red in H. subst.
+      left. exists x.2. red in H. subst.
       apply hadd. cbn. left. now destruct x.
       apply ih in H.
       intuition auto.
@@ -1822,11 +1390,11 @@ Section MoreNonEmpty.
     induction l.
     - cbn.
       split. intros x [->|] => //. reflexivity.
-      now exists t0; split => //.
+      now exists p; split => //.
     - destruct IHl as [ha hex].
       split.
       * intros x hin.
-        eapply (in_elt_inv x a [t0]) in hin as [<-|inih].
+        eapply (in_elt_inv x a [p]) in hin as [<-|inih].
         { cbn. rewrite fold_left_comm.
           { intros x' y z. rewrite assoc. now rewrite (comm (min_atom_value m y)) -assoc. }
           apply Zmin_opt_left. }
@@ -1863,8 +1431,8 @@ Section MoreNonEmpty.
 
   Lemma premise_min_spec_aux s k :
     premise_min s = k ->
-    (forall x, LevelExprSet.In x s -> (k <= x)%Z) /\
-    (exists x, LevelExprSet.In x s /\ k = x).
+    (forall x, LevelExprSet.In x s -> (k <= x.2)%Z) /\
+    (exists x, LevelExprSet.In x s /\ k = x.2).
   Proof.
     unfold premise_min.
     move: (to_nonempty_list_spec s).
@@ -1874,32 +1442,32 @@ Section MoreNonEmpty.
     induction l.
     - cbn.
       split. intros x [->|] => //. reflexivity.
-      now exists t0; split => //.
+      now exists p; split => //.
     - destruct IHl as [ha hex].
       split; intros.
-      eapply (in_elt_inv x a [t0]) in H as [<-|inih].
-      cbn. rewrite fold_left_comm. unfold level_expr_elt in *; lia. unfold level_expr_elt in *; lia.
+      eapply (in_elt_inv x a [p]) in H as [<-|inih].
+      cbn. rewrite fold_left_comm. lia. lia.
       specialize (ha _ inih).
       cbn. rewrite fold_left_comm. lia. lia.
       destruct hex as [minval [inmin ih]].
       cbn. rewrite fold_left_comm. lia.
-      destruct (Z.leb_spec a minval).
-      exists a. split; [intuition|]. rewrite -ih in H. unfold level_expr_elt in *; lia.
+      destruct (Z.leb_spec a.2 minval.2).
+      exists a. split; [intuition|]. rewrite -ih in H. lia.
       exists minval.
       cbn in inmin; split; [intuition auto|]. lia.
   Qed.
 
   Lemma premise_min_spec (s : nonEmptyLevelExprSet) :
-    (forall x, LevelExprSet.In x s -> premise_min s <= x) /\
-    (exists x, LevelExprSet.In x s /\ premise_min s = x).
+    (forall x, LevelExprSet.In x s -> premise_min s <= x.2) /\
+    (exists x, LevelExprSet.In x s /\ premise_min s = x.2).
   Proof.
     now apply premise_min_spec_aux.
   Qed.
 
   Lemma premise_max_spec_aux s k :
     premise_max s = k ->
-    (forall x, LevelExprSet.In x s -> x <= k) /\
-    (exists x, LevelExprSet.In x s /\ k = x).
+    (forall x, LevelExprSet.In x s -> x.2 <= k) /\
+    (exists x, LevelExprSet.In x s /\ k = x.2).
   Proof.
     unfold premise_max.
     move: (to_nonempty_list_spec s).
@@ -1909,24 +1477,25 @@ Section MoreNonEmpty.
     induction l.
     - cbn.
       split. intros x [->|] => //. reflexivity.
-      now exists t0; split => //.
+      now exists p; split => //.
     - destruct IHl as [ha hex].
       split; intros.
-      eapply (in_elt_inv x a [t0]) in H as [<-|inih].
-      cbn. rewrite fold_left_comm. unfold level_expr_elt in *; lia. unfold level_expr_elt in *; lia.
+      eapply (in_elt_inv x a [p]) in H as [<-|inih].
+      cbn. rewrite fold_left_comm. lia. lia.
       specialize (ha _ inih).
       cbn. rewrite fold_left_comm. lia. lia.
       destruct hex as [maxval [inmin ih]].
       cbn. rewrite fold_left_comm. lia.
-      destruct (Z.leb_spec a maxval).
-      exists maxval. cbn in inmin; split; [intuition auto|]. lia.
+      destruct (Z.leb_spec a.2 maxval.2).
+      exists maxval. cbn in inmin; split; [intuition auto|].
+      lia.
       exists a. split; [intuition|]. rewrite -ih in H. cbn in inmin.
-      unfold level_expr_elt in *; lia.
+      lia.
   Qed.
 
   Lemma premise_max_spec (s : nonEmptyLevelExprSet) :
-    (forall x, LevelExprSet.In x s -> x <= premise_max s) /\
-    (exists x, LevelExprSet.In x s /\ premise_max s = x).
+    (forall x, LevelExprSet.In x s -> x.2 <= premise_max s) /\
+    (exists x, LevelExprSet.In x s /\ premise_max s = x.2).
   Proof.
     now apply premise_max_spec_aux.
   Qed.
@@ -1975,12 +1544,12 @@ Section MoreNonEmpty.
     - cbn.
       intros eq.
       split. intros x [->|] => //. exists k. split => //. reflexivity.
-      now exists t0; split => //.
+      now exists p; split => //.
     - cbn. rewrite fold_left_comm. intros; apply fold_comm_assoc.
       intros heq. apply max_opt_spec in heq as [y' [z' [eqa [eqf ->]]]].
       specialize (IHl _ eqf). destruct IHl as [ha hex].
       split; intros.
-      eapply (in_elt_inv x a [t0]) in H as [<-|inih].
+      eapply (in_elt_inv x a [p]) in H as [<-|inih].
       { exists y'; intuition eauto. constructor; lia. }
       { specialize (ha _ inih) as [k' []]. exists k'; intuition eauto. constructor. depelim H0; lia. }
       destruct hex as [maxval [inmax ih]].
@@ -2001,7 +1570,7 @@ End MoreNonEmpty.
 
 Lemma min_premise_pos_spec {m prem k} :
   min_premise m prem = Some k ->
-  forall x, LevelExprSet.In x prem -> Some (levelexpr_k x + k)%Z ≤Z levelexpr_value m x.
+  forall x, LevelExprSet.In x prem -> Some (x.2 + k)%Z ≤Z levelexpr_value m x.
 Proof.
   pose proof (min_premise_spec m prem) as [amin [exmin [inminpre eqminpre]]].
   intros hprem x hin.
@@ -2124,7 +1693,7 @@ Definition check_model_invariants cls w m w' m' (modified : bool) :=
     [/\ w ⊂_lset w',
         w' ⊂_lset (LevelSet.union w (clauses_conclusions cls)),
         exists cl,
-          let cll := (levelexpr_level (concl cl)) in
+          let cll := (level (concl cl)) in
           [/\ Clauses.In cl cls, ~~ valid_clause m cl,
           LevelSet.In cll w' &
           opt_le Z.lt (level_value m cll) (level_value m' cll)],
@@ -2198,7 +1767,7 @@ Proof.
 Qed.
 
 Lemma min_atom_value_levelexpr_value m l a lv : min_atom_value m l = Some a -> levelexpr_value m l = Some lv ->
-  (a <= lv - l).
+  (a <= lv - l.2).
 Proof.
   destruct l as [l k]; cbn. unfold levelexpr_value. cbn. destruct level_value => //.
   intros [= <-] [= <-]. lia.
@@ -2450,10 +2019,10 @@ exists k',
   { induction l; cbn.
     - intros x y [= <-]. now eexists.
     - intros x y.
-      unfold min_atom_value, levelexpr_value, levelexpr_level. destruct a; cbn.
+      unfold min_atom_value, levelexpr_value, level. destruct a; cbn.
       destruct level_value => //=. eapply IHl. cbn. intros H'. exfalso.
       eapply H; eauto. }
-  - unfold min_atom_value, levelexpr_value, levelexpr_level. destruct t; cbn.
+  - unfold min_atom_value, levelexpr_value, level. destruct p; cbn.
     destruct level_value => //=. apply H0.
     intros; exfalso. now eapply H.
 Qed.
@@ -2527,10 +2096,10 @@ Proof.
     pose proof (min_atom_value_levelexpr_value m exmin).
     specialize (amax _ inminpre) as amax'. rewrite eqmaxpre in amax'.
     destruct amax' as [vexmin [eqexmin ltexmin]].
-    assert (expmin <= exmin). specialize (apmin _ inminpre). lia.
+    assert (expmin.2 <= exmin.2). specialize (apmin _ inminpre). lia.
     specialize (H4 _ _ eqminpre eqexmin). depelim ltexmin. etransitivity; tea.
     rewrite -eqmaxpre in H6. noconf H6.
-    unfold level_expr_elt in *. lia. }
+    lia. }
   transitivity (k + (maxpreml - (premise_min preml)))%Z. lia.
   (* assert (Z.of_nat (premise_min preml) <= maxpreml)%Z.
   { rewrite eqmaxpre.
@@ -2542,7 +2111,7 @@ Proof.
   enough (maxpreml <= (v_minus_w_bound W m))%Z. lia.
   { have vm := v_minus_w_bound_spec W m exmax. unfold levelexpr_value in eqmaxpre.
     rewrite -eqmaxpre in vm.
-    have [hlevels _] := (@levels_exprs_non_W_atoms W prem (levelexpr_level exmax)).
+    have [hlevels _] := (@levels_exprs_non_W_atoms W prem (level exmax)).
     rewrite levelexprset_levels_spec in hlevels.
     forward hlevels.
     exists exmax.2. now destruct exmax.
@@ -3781,8 +3350,8 @@ Section InnerLoop.
       pose proof (min_atom_value_levelexpr_value m exmin _ _ H2 lk').
       rewrite eqminpre H2. constructor. etransitivity; tea.
       rewrite eqmaxpre in eqmaxp.
-      assert (expmin <= exmin). specialize (apmin _ inminpre). lia.
-      unfold level_expr_elt in *. lia. }
+      assert (expmin.2 <= exmin.2). specialize (apmin _ inminpre). lia.
+      lia. }
     apply Z.leb_le. rewrite H1 in H2. depelim H2.
     transitivity (k + (maxpreml - premise_min preml)). lia.
     assert (Z.to_nat (gain (preml, (l, k))) <= max_gain clsdiff)%nat.
@@ -3798,7 +3367,7 @@ Section InnerLoop.
       (maxpreml + k - premise_min preml)) as ->. lia.
     assert (maxpreml <= v_minus_w_bound W m).
     { pose proof (v_minus_w_bound_spec W m exmax).
-      have [hlevels _] := (@levels_exprs_non_W_atoms W prem (levelexpr_level exmax)).
+      have [hlevels _] := (@levels_exprs_non_W_atoms W prem (level exmax)).
       rewrite levelexprset_levels_spec in hlevels.
       forward hlevels.
       exists exmax.2. now destruct exmax.
@@ -3975,7 +3544,7 @@ Section InnerLoop.
     check_model cls (w'', m) = Some (w', m') ->
     [/\ w'' ⊂_lset w', w' ⊂_lset (w'' ∪ w),
       exists cl : clause,
-        let cll := levelexpr_level (concl cl) in
+        let cll := level (concl cl) in
         [/\ Clauses.In cl cls, ~~ valid_clause m cl, LevelSet.In cll w'
           & (opt_le Z.lt (level_value m cll) (level_value m' cll))%Z]
       & model_extension w' m m'].
@@ -4586,8 +4155,7 @@ Section InnerLoop.
       apply levelmap_level_value_eq => k.
       rewrite model_update_spec. clear -mW om hin. firstorder.
     - subst x. apply levelmap_level_value_eq => k.
-      rewrite model_update_spec. cbn in *. firstorder. cbn in H.
-      apply om in incl as [x hm]. now apply H in hm.
+      rewrite model_update_spec. cbn in *. firstorder.
   Qed.
 
   Lemma strictly_updates_defined_model cls W m m' :
@@ -4722,7 +4290,7 @@ Section InnerLoop.
         { eapply model_map_outside_weaken. eapply hext. have incl := model_incl mr. lsets. }
         { apply hext. }
         eapply invalid_clause_measure in nvalid; tea.
-        exists (levelexpr_level (concl cll)).
+        exists (level (concl cll)).
         split => //.
         eapply clauses_conclusions_diff_left; tea.
         eapply clauses_conclusions_spec. exists cll; split => //. exact hind.
@@ -5729,7 +5297,7 @@ Proof.
     { destruct H1 as [cl [clcls nvalid hcll hv]].
       pose proof (model_ok mwc).
       eapply is_model_invalid_clause in H; tea.
-      assert (~ LevelSet.In (levelexpr_level (concl cl)) W).
+      assert (~ LevelSet.In (level (concl cl)) W).
       { intros hin. rewrite in_clauses_with_concl in H. intuition auto. }
       exists (concl cl). split => //. }
     rewrite -!diff_cardinal //. clear -w_incl clsV incl wcls_incl. have hincl := clauses_conclusions_levels cls. lsets. lsets.
@@ -6194,7 +5762,7 @@ Proof.
   destruct to_nonempty_list.
   pose proof to_nonempty_list_spec'.
   rewrite In_elements in H. rewrite -he in H. clear H0 he. clear -H.
-  destruct H. subst t.
+  destruct H. subst p.
   - induction l. cbn. auto.
     cbn. lia. cbn. lia.
   - induction l in H |- *.
@@ -7249,7 +6817,7 @@ Proof.
   rewrite {1}/min_premise.
   have hs' := to_nonempty_list_spec (add le prems).
   destruct to_nonempty_list.
-  have eqf : (fold_left (fun (min : option Z) (atom : LevelExpr.t) => option_map2 Z.min (min_atom_value m atom) min) l (min_atom_value m t)) =
+  have eqf : (fold_left (fun (min : option Z) (atom : LevelExpr.t) => option_map2 Z.min (min_atom_value m atom) min) l (min_atom_value m p)) =
     (option_map2 Z.min (min_atom_value m le) (min_premise m prems)).
   2:{ now rewrite eqf. }
   rewrite -(to_nonempty_list_spec' (add le prems)) in hs'. noconf hs'.
@@ -8101,15 +7669,9 @@ Module Abstract.
 End Abstract.
 End LoopCheckingImpl.
 
-Module LoopChecking
-  (* Signature of levels: decidable, ordered type *)
-  (Level : LevelOrderedType)
-  (LevelSet : LevelSet_fun Level)
-  (LevelExpr : LevelExprItf Level)
-  (LevelExprSet : LevelExprSet_fun Level LevelExpr)
-  (LevelMap : FMapOTInterface Level) <: LoopCheckingItf Level LevelSet LevelExpr LevelExprSet LevelMap.
-
-  Module Impl := LoopCheckingImpl(Level)(LevelSet)(LevelExpr)(LevelExprSet)(LevelMap).
+Module LoopChecking (LS : LevelSets).
+  Module Impl := LoopCheckingImpl(LS).
+  Import Impl.FLS.
 
   Definition model := Impl.Abstract.t.
 
