common/theories/LoopChecking/Common.v
@@ -1,0 +1,17 @@
+(* Distributed under the terms of the MIT license. *)
+From Stdlib Require Import ssreflect ssrbool ZArith.
+From Stdlib Require Import Program RelationClasses Morphisms.
+From Stdlib Require Import Orders OrderedTypeAlt OrderedTypeEx MSetList MSetInterface MSetAVL MSetFacts FMapInterface MSetProperties MSetDecide.
+From MetaRocq.Utils Require Import utils.
+
+From MetaRocq.Common Require Universes.
+From Equations Require Import Equations.
+Set Equations Transparent.
+
+Ltac rw l := rewrite_strat (topdown l).
+Ltac rw_in l H := rewrite_strat (topdown l) in H.
+
+
+(* TODO move *)
+Arguments exist {A P}.
+Definition inspect {A} (x : A) : { y : A | x = y } := exist x eq_refl.
