common/theories/LoopChecking/Interfaces.v
@@ -1,0 +1,433 @@
+(* Distributed under the terms of the MIT license. *)
+From Stdlib Require Import ssreflect ssrbool ZArith.
+From Stdlib Require Import Program RelationClasses Morphisms.
+From Stdlib Require Import Orders OrderedTypeAlt OrderedTypeEx MSetList MSetInterface MSetAVL MSetFacts FMapInterface MSetProperties MSetDecide.
+From MetaRocq.Utils Require Import utils.
+
+From MetaRocq.Common Require Universes.
+From MetaRocq.Common Require Import LoopChecking.Common.
+From Equations Require Import Equations.
+Set Equations Transparent.
+
+Module FMapOrderedType_from_UsualOrderedType (O : UsualOrderedType).
+  Import O.
+  Definition t := O.t.
+  Definition eq : O.t -> O.t -> Prop := O.eq.
+  Definition lt : O.t -> O.t -> Prop := O.lt.
+  Definition eq_refl : forall x : O.t, eq x x := reflexivity.
+  Definition eq_sym : forall x y : O.t, eq x y -> eq y x := fun x y H => symmetry H.
+
+  Lemma eq_trans : forall x y z, O.eq x y -> O.eq y z -> O.eq x z.
+  Proof. intros x y z. unfold O.eq. apply transitivity. Qed.
+  Lemma lt_trans : forall x y z, O.lt x y -> O.lt y z -> O.lt x z.
+  Proof. intros. eapply O.lt_strorder; tea. Qed.
+
+  Lemma lt_not_eq : forall x y : O.t, lt x y -> ~ eq x y.
+  Proof.
+    intros x y H eq. do 2 red in eq. subst x. now eapply lt_strorder in H.
+  Qed.
+
+  Definition compare : forall x y : O.t, Compare lt eq x y.
+  Proof.
+    intros.
+    case_eq (compare x y); intros.
+    apply EQ. abstract (destruct (compare_spec x y) => //).
+    apply LT. abstract (destruct (compare_spec x y) => //).
+    apply GT. abstract (destruct (compare_spec x y) => //).
+  Defined.
+
+  Definition eq_dec : forall x y : O.t, {eq x y} + {~ eq x y} := eq_dec.
+End FMapOrderedType_from_UsualOrderedType.
+
+Module Type LevelOrderedType.
+  Include UsualOrderedType.
+
+  Parameter reflect_eq : ReflectEq t.
+  #[local] Existing Instance reflect_eq.
+  Parameter eq_leibniz : forall (x y : t), eq x y -> x = y.
+
+  Parameter to_string : t -> string.
+
+End LevelOrderedType.
+
+Module Type FMapOTInterface (E : UsualOrderedType).
+  Module OT := FMapOrderedType_from_UsualOrderedType E.
+  Include FMapInterface.Sfun OT.
+End FMapOTInterface.
+
+Module Type LevelSet_fun (Level : LevelOrderedType).
+  Include SWithLeibniz with Module E := Level.
+End LevelSet_fun.
+
+Module Type LevelExprItf (Level : LevelOrderedType).
+  Include UsualOrderedType with Definition t := (Level.t * Z)%type.
+  Parameter eq_leibniz : forall (x y : t), eq x y -> x = y.
+End LevelExprItf.
+
+Module Type LevelExprSet_fun (Level : LevelOrderedType) (LevelExpr : LevelExprItf Level).
+  Include SWithLeibniz with Module E := LevelExpr.
+
+  Record nonEmptyLevelExprSet
+    := { t_set :> t ;
+          t_ne  : is_empty t_set = false }.
+
+End LevelExprSet_fun.
+
+Module Type LevelSets.
+  (* Signature of levels: decidable, ordered type *)
+  Declare Module Import Level : LevelOrderedType.
+  Declare Module Import LevelSet : LevelSet_fun Level.
+  Declare Module Import LevelExpr : LevelExprItf Level.
+  Declare Module Import LevelExprSet : LevelExprSet_fun Level LevelExpr.
+  Declare Module Import LevelMap : FMapOTInterface Level.
+End LevelSets.
+
+
+Module FromLevelSets (LS : LevelSets).
+  Export LS.
+
+  Definition level (e : LevelExpr.t) : Level.t := fst e.
+  Coercion level : LevelExpr.t >-> Level.t.
+  Extraction Inline level.
+
+  Definition levels (e : LevelExprSet.t) :=
+  LevelExprSet.fold (fun le => LevelSet.add (level le)) e LevelSet.empty.
+  Export LevelExprSet (nonEmptyLevelExprSet, t_set, t_ne).
+
+  Existing Instance Level.reflect_eq.
+
+  Module LevelSetFact := WFactsOn Level LevelSet.
+  Module LevelSetProp := WPropertiesOn Level LevelSet.
+  Module LevelSetDecide := LevelSetProp.Dec.
+  Module LevelMapFact := FMapFacts.WProperties_fun LevelMap.OT LevelMap.
+
+  Ltac lsets := LevelSetDecide.fsetdec.
+  Notation "(=_lset)" := LevelSet.Equal (at level 0).
+  Infix "=_lset" := LevelSet.Equal (at level 30).
+  Infix "⊂_lset" := LevelSet.Subset (at level 70).
+  Infix "∪" := LevelSet.union (at level 70).
+
+
+Definition print_level_nat_map (m : LevelMap.t nat) :=
+  let list := LevelMap.elements m in
+  print_list (fun '(l, w) => Level.to_string l ^ " -> " ^ string_of_nat w) nl list.
+
+Definition print_lset (l : LevelSet.t) :=
+  let list := LevelSet.elements l in
+  print_list Level.to_string " " list.
+
+Module LevelExprSetFact := WFactsOn LevelExpr LevelExprSet.
+Module LevelExprSetProp := WPropertiesOn LevelExpr LevelExprSet.
+
+(* We have decidable equality w.r.t leibniz equality for sets of levels. *)
+#[global, program] Instance levelexprset_reflect : ReflectEq LevelExprSet.t :=
+  { eqb := LevelExprSet.equal }.
+Next Obligation.
+  destruct (LevelExprSet.equal x y) eqn:e; constructor.
+  eapply LevelExprSet.equal_spec in e.
+  now eapply LevelExprSet.eq_leibniz.
+  intros e'.
+  subst y.
+  pose proof (@LevelExprSetFact.equal_1 x x).
+  forward H. reflexivity. congruence.
+Qed.
+
+#[global] Instance levelexprset_eq_dec : Classes.EqDec LevelExprSet.t := Classes.eq_dec.
+
+Derive NoConfusion for LevelExprSet.nonEmptyLevelExprSet.
+
+(* We use uip on the is_empty condition *)
+#[global, program] Instance nonEmptyLevelExprSet_reflect : ReflectEq nonEmptyLevelExprSet :=
+  { eqb x y := eqb x.(t_set) y.(t_set) }.
+Next Obligation.
+  destruct (eqb_spec (t_set x) (t_set y)); constructor.
+  destruct x, y; cbn in *. subst.
+  now rewrite (uip t_ne0 t_ne1).
+  intros e; subst x; apply H.
+  reflexivity.
+Qed.
+
+(** This coercion allows to see the non-empty set as a regular [LevelExprSet.t] *)
+Coercion t_set : nonEmptyLevelExprSet >-> LevelExprSet.t.
+Module LevelExprSetDecide := WDecide (LevelExprSet).
+Ltac lesets := LevelExprSetDecide.fsetdec.
+Infix "⊂_leset" := LevelExprSet.Subset (at level 70).
+
+Lemma levelset_not_Empty_is_empty s :
+  LevelSet.is_empty s = false <-> ~ LevelSet.Empty s.
+Proof.
+  split.
+  - intros H he. red in he. apply negbT in H. unshelve eapply (contraNnot _ H).
+    3:exact he. intros ha. now apply LevelSetFact.is_empty_1.
+  - intros ne. destruct LevelSet.is_empty eqn:he => //.
+    eapply LevelSetFact.is_empty_2 in he. contradiction.
+Qed.
+
+Module NonEmptySetFacts.
+  #[program] Definition singleton (e : LevelExpr.t) : nonEmptyLevelExprSet
+    := {| t_set := LevelExprSet.singleton e |}.
+  Next Obligation.
+    apply negbTE.
+    eapply (contra_notN (P := LevelExprSet.Empty (LevelExprSet.singleton e))).
+    apply LevelExprSetFact.is_empty_2. intros ne. red in ne. specialize (ne e). lesets.
+  Qed.
+
+  Lemma not_Empty_is_empty s :
+    ~ LevelExprSet.Empty s <-> LevelExprSet.is_empty s = false.
+  Proof.
+    split.
+    - intro H. apply not_true_is_false. intro H'.
+      apply H. now apply LevelExprSetFact.is_empty_2 in H'.
+    - intros H he. red in he. apply negbT in H. unshelve eapply (contraNnot _ H).
+      3:exact he. intros ha. now apply LevelExprSetFact.is_empty_1.
+  Qed.
+
+  Program Definition add (e : LevelExpr.t) (u : nonEmptyLevelExprSet) : nonEmptyLevelExprSet
+    := {| t_set := LevelExprSet.add e u |}.
+  Next Obligation.
+    apply not_Empty_is_empty; intro H.
+    eapply H. eapply LevelExprSet.add_spec.
+    left; reflexivity.
+  Qed.
+
+  Lemma add_spec e u e' :
+    LevelExprSet.In e' (add e u) <-> e' = e \/ LevelExprSet.In e' u.
+  Proof.
+    apply LevelExprSet.add_spec.
+  Qed.
+
+  Definition add_list : list LevelExpr.t -> nonEmptyLevelExprSet -> nonEmptyLevelExprSet
+    := List.fold_left (fun u e => add e u).
+
+  Lemma add_list_spec l u e :
+    LevelExprSet.In e (add_list l u) <-> In e l \/ LevelExprSet.In e u.
+  Proof.
+    unfold add_list. rewrite <- fold_left_rev_right.
+    etransitivity. 2:{ eapply or_iff_compat_r. etransitivity.
+                        2: apply @InA_In_eq with (A:=LevelExpr.t).
+                        eapply InA_rev. }
+    induction (List.rev l); cbn.
+    - split. intuition. intros [H|H]; tas. invs H.
+    - split.
+      + intro H. apply add_spec in H. destruct H as [H|H].
+        * left. now constructor.
+        * apply IHl0 in H. destruct H as [H|H]; [left|now right].
+          now constructor 2.
+      + intros [H|H]. inv H.
+        * apply add_spec; now left.
+        * apply add_spec; right. apply IHl0. now left.
+        * apply add_spec; right. apply IHl0. now right.
+  Qed.
+
+  Lemma elements_not_empty {u : nonEmptyLevelExprSet} : LevelExprSet.elements u <> [].
+  Proof.
+    rewrite -LevelExprSetProp.elements_Empty.
+    move/LevelExprSetFact.is_empty_1.
+    destruct u as [u1 u2]; cbn in *. congruence.
+  Qed.
+
+  Equations to_nonempty_list (u : nonEmptyLevelExprSet) : LevelExpr.t * list LevelExpr.t :=
+  | u with inspect (LevelExprSet.elements u) := {
+    | exist [] eqel => False_rect _ (elements_not_empty eqel)
+    | exist (e :: l) _ => (e, l) }.
+
+  Lemma singleton_to_nonempty_list e : to_nonempty_list (singleton e) = (e, []).
+  Proof.
+    funelim (to_nonempty_list (singleton e)). bang.
+    clear H.
+    pose proof (LevelExprSet.singleton_spec e1 e).
+    rewrite LevelExprSetFact.elements_iff in H.
+    rewrite InA_In_eq in H. rewrite e0 in H.
+    destruct H. forward H. now left. noconf H. f_equal.
+    pose proof (LevelExprSet.cardinal_spec (LevelExprSet.singleton e1)). rewrite e0 in H. cbn in H.
+    rewrite LevelExprSetProp.singleton_cardinal in H.
+    destruct l => //.
+  Qed.
+
+  Lemma to_nonempty_list_spec u :
+    let '(e, u') := to_nonempty_list u in
+    e :: u' = LevelExprSet.elements u.
+  Proof.
+    funelim (to_nonempty_list u). bang. now rewrite e0.
+  Qed.
+
+  Lemma to_nonempty_list_spec' u :
+    (to_nonempty_list u).1 :: (to_nonempty_list u).2 = LevelExprSet.elements u.
+  Proof.
+    pose proof (to_nonempty_list_spec u).
+    now destruct (to_nonempty_list u).
+  Qed.
+
+  Lemma In_to_nonempty_list (u : nonEmptyLevelExprSet) (e : LevelExpr.t) :
+    LevelExprSet.In e u
+    <-> e = (to_nonempty_list u).1 \/ In e (to_nonempty_list u).2.
+  Proof.
+    etransitivity. symmetry. apply LevelExprSet.elements_spec1.
+    pose proof (to_nonempty_list_spec' u) as H.
+    destruct (to_nonempty_list u) as [e' l]; cbn in *.
+    rewrite <- H; clear. etransitivity. apply InA_cons.
+    eapply or_iff_compat_l. apply InA_In_eq.
+  Qed.
+
+  Lemma In_to_nonempty_list_rev (u : nonEmptyLevelExprSet) (e : LevelExpr.t) :
+    LevelExprSet.In e u
+    <-> e = (to_nonempty_list u).1 \/ In e (List.rev (to_nonempty_list u).2).
+  Proof.
+    etransitivity. eapply In_to_nonempty_list.
+    apply or_iff_compat_l. apply in_rev.
+  Qed.
+
+  Program Definition map (f : LevelExpr.t -> LevelExpr.t) (u : nonEmptyLevelExprSet) : nonEmptyLevelExprSet :=
+    {| t_set := LevelExprSetProp.of_list (List.map f (LevelExprSet.elements u)) |}.
+  Next Obligation.
+    have hs := to_nonempty_list_spec u.
+    destruct (to_nonempty_list u). rewrite -hs. cbn.
+    apply not_Empty_is_empty => he. apply (he (f t)).
+    lesets.
+  Qed.
+
+  Lemma map_spec f u e :
+    LevelExprSet.In e (map f u) <-> exists e0, LevelExprSet.In e0 u /\ e = (f e0).
+  Proof.
+    unfold map; cbn.
+    rewrite LevelExprSetProp.of_list_1 InA_In_eq in_map_iff.
+    split.
+    - intros [x [<- hin]]. exists x. split => //.
+      rewrite -InA_In_eq in hin. now apply LevelExprSet.elements_spec1 in hin.
+    - intros [x [hin ->]]. exists x. split => //.
+      rewrite -InA_In_eq. now apply LevelExprSet.elements_spec1.
+  Qed.
+
+  Program Definition non_empty_union (u v : nonEmptyLevelExprSet) : nonEmptyLevelExprSet :=
+    {| t_set := LevelExprSet.union u v |}.
+  Next Obligation.
+    apply not_Empty_is_empty; intro H.
+    assert (HH: LevelExprSet.Empty u). {
+      intros x Hx. apply (H x).
+      eapply LevelExprSet.union_spec. now left. }
+    apply LevelExprSetFact.is_empty_1 in HH.
+    rewrite t_ne in HH; discriminate.
+  Qed.
+
+
+  Lemma eq_univ (u v : nonEmptyLevelExprSet) :
+    u = v :> LevelExprSet.t -> u = v.
+  Proof.
+    destruct u as [u1 u2], v as [v1 v2]; cbn. intros X; destruct X.
+    now rewrite (uip_bool _ _ u2 v2).
+  Qed.
+
+  Lemma eq_univ_equal (u v : nonEmptyLevelExprSet) :
+    LevelExprSet.Equal u v <-> u = v.
+  Proof.
+    split.
+    - intro H. now apply eq_univ, LevelExprSet.eq_leibniz.
+    - intros ->; reflexivity.
+  Qed.
+
+  Lemma eq_univ_elements (u v : nonEmptyLevelExprSet) :
+    LevelExprSet.elements u = LevelExprSet.elements v -> u = v.
+  Proof.
+    intro H. apply eq_univ.
+    destruct u as [u1 u2], v as [v1 v2]; cbn in *; clear u2 v2.
+    eapply LevelExprSet.eq_leibniz. red.
+    intros x. rewrite -!LevelExprSet.elements_spec1 H //.
+  Qed.
+
+  Lemma univ_expr_eqb_true_iff (u v : nonEmptyLevelExprSet) :
+    LevelExprSet.equal u v <-> u = v.
+  Proof.
+    split.
+    - intros.
+      apply eq_univ_equal. now apply LevelExprSet.equal_spec.
+    - intros ->. now apply LevelExprSet.equal_spec.
+  Qed.
+
+  Lemma univ_expr_eqb_comm (u v : nonEmptyLevelExprSet) :
+    LevelExprSet.equal u v <-> LevelExprSet.equal v u.
+  Proof.
+    transitivity (u = v). 2: transitivity (v = u).
+    - apply univ_expr_eqb_true_iff.
+    - split; apply eq_sym.
+    - split; apply univ_expr_eqb_true_iff.
+  Qed.
+
+
+  Lemma LevelExprSet_for_all_false f u :
+    LevelExprSet.for_all f u = false -> LevelExprSet.exists_ (negb ∘ f) u.
+  Proof.
+    intro H. rewrite LevelExprSetFact.exists_b.
+    rewrite LevelExprSetFact.for_all_b in H.
+    all: try now intros x y [].
+    induction (LevelExprSet.elements u); cbn in *; [discriminate|].
+    apply andb_false_iff in H; apply orb_true_iff; destruct H as [H|H].
+    left; now rewrite H.
+    right; now rewrite IHl.
+  Qed.
+
+  Lemma LevelExprSet_For_all_exprs (P : LevelExpr.t -> Prop) (u : nonEmptyLevelExprSet)
+    : LevelExprSet.For_all P u
+      <-> P (to_nonempty_list u).1 /\ Forall P (to_nonempty_list u).2.
+  Proof.
+    etransitivity.
+    - eapply iff_forall; intro e. eapply imp_iff_compat_r.
+      apply In_to_nonempty_list.
+    - cbn; split.
+      + intro H. split. apply H. now left.
+        apply Forall_forall. intros x H0.  apply H; now right.
+      + intros [H1 H2] e [He|He]. subst e; tas.
+        eapply Forall_forall in H2; tea.
+  Qed.
+
+  Lemma add_comm {le le' e} : add le (add le' e) = add le' (add le e).
+  Proof.
+    apply eq_univ_equal. intros x.
+    rewrite !LevelExprSet.add_spec. firstorder.
+  Qed.
+
+  #[program]
+  Definition univ_union (prems prems' : nonEmptyLevelExprSet) : nonEmptyLevelExprSet :=
+    {| t_set := LevelExprSet.union prems prems' |}.
+  Next Obligation.
+    destruct prems, prems'; cbn.
+    destruct (LevelExprSet.is_empty (LevelExprSet.union _ _)) eqn:ise => //.
+    eapply LevelExprSetFact.is_empty_2 in ise.
+    eapply not_Empty_is_empty in t_ne0, t_ne1.
+    destruct t_ne0. lesets.
+  Qed.
+
+  Lemma univ_union_spec u u' l :
+    LevelExprSet.In l (univ_union u u') <->
+    LevelExprSet.In l u \/ LevelExprSet.In l u'.
+  Proof.
+    destruct u, u'; unfold univ_union; cbn.
+    apply LevelExprSet.union_spec.
+  Qed.
+
+  Lemma univ_union_add_singleton u le : univ_union u (singleton le) = add le u.
+  Proof.
+    apply eq_univ_equal.
+    intros x. rewrite univ_union_spec LevelExprSet.singleton_spec add_spec.
+    intuition auto.
+  Qed.
+
+  Lemma univ_union_comm {u u'} : univ_union u u' = univ_union u' u.
+  Proof.
+    apply eq_univ_equal.
+    intros x. rewrite !univ_union_spec.
+    intuition auto.
+  Qed.
+
+  Lemma univ_union_add_distr {le u u'} : univ_union (add le u) u' = add le (univ_union u u').
+  Proof.
+    apply eq_univ_equal.
+    intros x. rewrite !univ_union_spec !add_spec !univ_union_spec.
+    intuition auto.
+  Qed.
+
+End NonEmptySetFacts.
+Export NonEmptySetFacts.
+
+
+
+End FromLevelSets.
